Coq Developments/msci/GV_Typing.v
@@ -32,13 +32,37 @@ Proof.
               end.
 Qed.
 
-Lemma wt_tm_is_lc : forall Φ t T
-    (WT: Φ ⊢ t ∈ T),
-  lc t.
+Lemma wt_tm_is_lc:
+  forall Φ t T
+         (WT: Φ ⊢ t ∈ T),
+    lc t.
 Proof.
   ii; induction WT; des_wfs; match goal with
                                | [H: are_dual ?S ?dS |- _] =>
                                  apply duals_are_wf in H; des
                                | |- _ => idtac
                              end; eauto using subst_lc.
+Qed.
+
+Lemma gv_in_env_fv_1:
+  forall Φ M T x
+         (WT: Φ ⊢ M ∈ T)
+         (IN: x `in` dom Φ),
+    x `in` GVFV M.
+Proof.
+  ii; induction WT; try (by s; simpl_env in *; destruct_in; auto).
+  - pick fresh y; destruct_notin; find_specializes; s; des.
+    simpl_env in *; destruct_in; apply open_fv_proc_1 in H; auto.
+  - pick fresh y; pick fresh z; destruct_notin.
+    apply notin_singleton_2 in NotInTac1.
+    forwards NIN: notin_union_3 Fr0 NotInTac1.
+    specializes H Fr NIN.
+    simpl_env in *; destruct_in; s; [fsetdec|].
+    do 2 !apply open_fv_proc_1 in H; auto.
+  - pick fresh y; destruct_notin; find_specializes; s.
+    simpl_env in *; destruct_in; auto.
+    apply open_fv_proc_1 in H; auto.
+  - pick fresh y; destruct_notin; find_specializes; s.
+    simpl_env in *; destruct_in; solve [apply open_fv_proc_1 in H; auto
+                                       |apply open_fv_proc_1 in H0; auto].
 Qed.
